up to declarative typing

theories/AutoSubst/PiUniv.sig
@@ -1,0 +1,8 @@
+sort : Type
+aname : Type
+term : Type
+
+tSort : sort -> term
+tProd : aname -> term -> (bind term in term) -> term
+tLambda : aname -> term -> (bind term in term) -> term
+tApp : term -> term -> term
