theories/Weakening.v
@@ -1,52 +1,56 @@
-From MetaCoq.PCUIC Require Import PCUICAst PCUICRenameConv PCUICSigmaCalculus PCUICInstConv.
-From LogRel Require Import Notations Untyped.
+From Coq Require Import Lia.
+From LogRel.AutoSubst Require Import core unscoped Ast.
+From LogRel Require Import Utils BasicAst Notations Context Untyped.
 
 Inductive weakening : Set :=
   | wk_id : weakening
   | wk_step (w : weakening) : weakening
-  | wk_lift (w : weakening) : weakening.
+  | wk_up (w : weakening) : weakening.
 
 (* Transforms an (intentional) weakening into a renaming *)
 Fixpoint wk_to_ren (ρ : weakening) : nat -> nat :=
   match ρ with
-    | wk_id => ren_id
-    | wk_step ρ' => S ∘ (wk_to_ren ρ')
-    | wk_lift ρ' => shiftn 1 (wk_to_ren ρ')
+    | wk_id => id
+    | wk_step ρ' => (wk_to_ren ρ') >> S
+    | wk_up ρ' => up_ren (wk_to_ren ρ')
   end.
 Coercion wk_to_ren : weakening >-> Funclass.
+
+#[global] Instance RenWk_term : (Ren1 weakening term term) :=
+  fun ρ t => ren_term (wk_to_ren ρ) t.
 
 Inductive well_weakening : weakening -> context -> context -> Type :=
   | well_id (Γ : context) : well_weakening wk_id Γ Γ
   | well_step (Γ Δ : context) (na : aname) (A : term) (ρ : weakening) :
     well_weakening ρ Γ Δ -> well_weakening (wk_step ρ) (Γ,,vass na A) Δ
-  | well_lift (Γ Δ : context) (na : aname) (A : term) (ρ : weakening) :
-    well_weakening ρ Γ Δ -> well_weakening (wk_lift ρ) (Γ,,vass na (A.[ren ρ])) (Δ,, vass na A).
+  | well_up (Γ Δ : context) (na : aname) (A : term) (ρ : weakening) :
+    well_weakening ρ Γ Δ -> well_weakening (wk_up ρ) (Γ,,vass na A⟨ρ⟩) (Δ,, vass na A).
 
 Fixpoint wk_compose (ρ ρ' : weakening) : weakening :=
   match ρ, ρ' with
     | wk_id, _ => ρ'
     | wk_step ν , _ => wk_step (wk_compose ν ρ')
-    | wk_lift ν, wk_id => ρ
-    | wk_lift ν, wk_step ν' => wk_step (wk_compose ν ν')
-    | wk_lift ν, wk_lift ν' => wk_lift (wk_compose ν ν')
+    | wk_up ν, wk_id => ρ
+    | wk_up ν, wk_step ν' => wk_step (wk_compose ν ν')
+    | wk_up ν, wk_up ν' => wk_up (wk_compose ν ν')
   end.
 
-Lemma wk_compose_compose (ρ ρ' : weakening) : (wk_compose ρ ρ' : nat -> nat) =1 ρ ∘ ρ'.
+Lemma wk_compose_compose (ρ ρ' : weakening) : wk_to_ren (wk_compose ρ ρ') =1 ρ' >> ρ.
 Proof.
   induction ρ in ρ' |- *.
   - reflexivity.
   - cbn.
-    intros ?.
-    now rewrite IHρ.
+    rewrite IHρ.
+    now fsimpl.
   - destruct ρ'.
     + reflexivity.
-    + intros n.
-      cbn.
-      now rewrite IHρ, Nat.sub_0_r.
-    + intros [] ; cbn.
-      1: reflexivity.
-      repeat rewrite Nat.sub_0_r.
-      now rewrite IHρ.
+    + cbn.
+      rewrite IHρ.
+      now asimpl.
+    + cbn.
+      asimpl.
+      rewrite IHρ.
+      now asimpl.
 Qed.
 
 Lemma well_wk_compose {ρ ρ' : weakening} {Δ Δ' Δ'' : context} :
@@ -56,13 +60,13 @@ Proof.
   induction H as [| | ? ? ? ? ν] in ρ', Δ'', H' |- *.
   all: cbn.
   - eassumption.
-  - now econstructor.
-  - inversion H' as [| | ? ? na' A' ν'] ; subst ; clear H'.
-    1-2: now econstructor.
-    rewrite inst_assoc.
-    replace (A'.[ren ν' ∘s ren ν]) with (A'.[ren (wk_compose ν ν')]) by
-      now rewrite compose_ren, wk_compose_compose.
-    now econstructor.
+  - econstructor. auto.
+  - inversion H' as [| | ? ? na' A' ν']; subst ; clear H'.
+    1-2: now econstructor ; auto.
+    asimpl.
+    replace (ren_term (ν' >> ν) A') with (ren_term (wk_compose ν ν') A')
+      by now rewrite wk_compose_compose.
+    econstructor ; auto.
 Qed.
 
 #[projections(primitive)]Record wk_well_wk {Γ Δ : context} :=
@@ -73,10 +77,12 @@ Notation "Γ ≤ Δ" := (wk_well_wk Γ Δ).
 
 #[global] Hint Resolve well_wk : core.
 
+#[global] Instance RenWlWk_term {Γ Δ : context }: (Ren1 (Γ ≤ Δ) term term) :=
+  fun ρ t => ren_term (wk_to_ren ρ.(wk)) t.
+
 Definition wk_well_wk_compose {Γ Γ' Γ'' : context} (ρ : Γ ≤ Γ') (ρ' : Γ' ≤ Γ'') : Γ ≤ Γ'' :=
   {| wk := wk_compose ρ.(wk) ρ'.(wk) ; well_wk := well_wk_compose ρ.(well_wk) ρ'.(well_wk) |}.
 Notation "ρ ∘w ρ'" := (wk_well_wk_compose ρ ρ').
-
 
 Lemma well_length {Γ Δ : context} (ρ : Γ ≤ Δ) : #|Δ| <= #|Γ|.
 Proof.
@@ -86,7 +92,7 @@ Proof.
 Qed.
 
 (* Testing that the definitions are right *)
-Lemma id_ren (Γ : context) (ρ : Γ ≤ Γ) : (wk_to_ren ρ) =1 ren_id.
+Lemma id_ren (Γ : context) (ρ : Γ ≤ Γ) : (wk_to_ren ρ) =1 id.
 Proof.
   destruct ρ as [ρ wellρ].
   cbn in *.
@@ -99,7 +105,8 @@ Proof.
   - reflexivity.
   - pose proof (well_length {| wk := ρ ; well_wk := wellρ |}).
     now cbn in * ; lia.
-  - etransitivity.
-    2: eapply shiftn_id.
-    now rewrite IHwellρ.
+  - asimpl.
+    setoid_rewrite IHwellρ.
+    2: now cbn in * ; lia.
+    now intros [] ; reflexivity.
 Qed.
