theories/AutoSubst/Ast.v
@@ -1,0 +1,928 @@
+From LogRel.AutoSubst Require Import core unscoped.
+From LogRel Require Import BasicAst.
+Require Import Setoid Morphisms Relation_Definitions.
+
+
+Module Core.
+
+Inductive term : Type :=
+  | tRel : nat -> term
+  | tSort : sort -> term
+  | tProd : aname -> term -> term -> term
+  | tLambda : aname -> term -> term -> term
+  | tApp : term -> term -> term.
+
+Lemma congr_tSort {s0 : sort} {t0 : sort} (H0 : s0 = t0) :
+  tSort s0 = tSort t0.
+Proof.
+exact (eq_trans eq_refl (ap (fun x => tSort x) H0)).
+Qed.
+
+Lemma congr_tProd {s0 : aname} {s1 : term} {s2 : term} {t0 : aname}
+  {t1 : term} {t2 : term} (H0 : s0 = t0) (H1 : s1 = t1) (H2 : s2 = t2) :
+  tProd s0 s1 s2 = tProd t0 t1 t2.
+Proof.
+exact (eq_trans
+         (eq_trans (eq_trans eq_refl (ap (fun x => tProd x s1 s2) H0))
+            (ap (fun x => tProd t0 x s2) H1))
+         (ap (fun x => tProd t0 t1 x) H2)).
+Qed.
+
+Lemma congr_tLambda {s0 : aname} {s1 : term} {s2 : term} {t0 : aname}
+  {t1 : term} {t2 : term} (H0 : s0 = t0) (H1 : s1 = t1) (H2 : s2 = t2) :
+  tLambda s0 s1 s2 = tLambda t0 t1 t2.
+Proof.
+exact (eq_trans
+         (eq_trans (eq_trans eq_refl (ap (fun x => tLambda x s1 s2) H0))
+            (ap (fun x => tLambda t0 x s2) H1))
+         (ap (fun x => tLambda t0 t1 x) H2)).
+Qed.
+
+Lemma congr_tApp {s0 : term} {s1 : term} {t0 : term} {t1 : term}
+  (H0 : s0 = t0) (H1 : s1 = t1) : tApp s0 s1 = tApp t0 t1.
+Proof.
+exact (eq_trans (eq_trans eq_refl (ap (fun x => tApp x s1) H0))
+         (ap (fun x => tApp t0 x) H1)).
+Qed.
+
+Lemma upRen_term_term (xi : nat -> nat) : nat -> nat.
+Proof.
+exact (up_ren xi).
+Defined.
+
+Fixpoint ren_term (xi_term : nat -> nat) (s : term) {struct s} : term :=
+  match s with
+  | tRel s0 => tRel (xi_term s0)
+  | tSort s0 => tSort s0
+  | tProd s0 s1 s2 =>
+      tProd s0 (ren_term xi_term s1) (ren_term (upRen_term_term xi_term) s2)
+  | tLambda s0 s1 s2 =>
+      tLambda s0 (ren_term xi_term s1)
+        (ren_term (upRen_term_term xi_term) s2)
+  | tApp s0 s1 => tApp (ren_term xi_term s0) (ren_term xi_term s1)
+  end.
+
+Lemma up_term_term (sigma : nat -> term) : nat -> term.
+Proof.
+exact (scons (tRel var_zero) (funcomp (ren_term shift) sigma)).
+Defined.
+
+Fixpoint subst_term (sigma_term : nat -> term) (s : term) {struct s} : 
+term :=
+  match s with
+  | tRel s0 => sigma_term s0
+  | tSort s0 => tSort s0
+  | tProd s0 s1 s2 =>
+      tProd s0 (subst_term sigma_term s1)
+        (subst_term (up_term_term sigma_term) s2)
+  | tLambda s0 s1 s2 =>
+      tLambda s0 (subst_term sigma_term s1)
+        (subst_term (up_term_term sigma_term) s2)
+  | tApp s0 s1 => tApp (subst_term sigma_term s0) (subst_term sigma_term s1)
+  end.
+
+Lemma upId_term_term (sigma : nat -> term)
+  (Eq : forall x, sigma x = tRel x) :
+  forall x, up_term_term sigma x = tRel x.
+Proof.
+exact (fun n =>
+       match n with
+       | S n' => ap (ren_term shift) (Eq n')
+       | O => eq_refl
+       end).
+Qed.
+
+Fixpoint idSubst_term (sigma_term : nat -> term)
+(Eq_term : forall x, sigma_term x = tRel x) (s : term) {struct s} :
+subst_term sigma_term s = s :=
+  match s with
+  | tRel s0 => Eq_term s0
+  | tSort s0 => congr_tSort (eq_refl s0)
+  | tProd s0 s1 s2 =>
+      congr_tProd (eq_refl s0) (idSubst_term sigma_term Eq_term s1)
+        (idSubst_term (up_term_term sigma_term) (upId_term_term _ Eq_term) s2)
+  | tLambda s0 s1 s2 =>
+      congr_tLambda (eq_refl s0) (idSubst_term sigma_term Eq_term s1)
+        (idSubst_term (up_term_term sigma_term) (upId_term_term _ Eq_term) s2)
+  | tApp s0 s1 =>
+      congr_tApp (idSubst_term sigma_term Eq_term s0)
+        (idSubst_term sigma_term Eq_term s1)
+  end.
+
+Lemma upExtRen_term_term (xi : nat -> nat) (zeta : nat -> nat)
+  (Eq : forall x, xi x = zeta x) :
+  forall x, upRen_term_term xi x = upRen_term_term zeta x.
+Proof.
+exact (fun n => match n with
+                | S n' => ap shift (Eq n')
+                | O => eq_refl
+                end).
+Qed.
+
+Fixpoint extRen_term (xi_term : nat -> nat) (zeta_term : nat -> nat)
+(Eq_term : forall x, xi_term x = zeta_term x) (s : term) {struct s} :
+ren_term xi_term s = ren_term zeta_term s :=
+  match s with
+  | tRel s0 => ap (tRel) (Eq_term s0)
+  | tSort s0 => congr_tSort (eq_refl s0)
+  | tProd s0 s1 s2 =>
+      congr_tProd (eq_refl s0) (extRen_term xi_term zeta_term Eq_term s1)
+        (extRen_term (upRen_term_term xi_term) (upRen_term_term zeta_term)
+           (upExtRen_term_term _ _ Eq_term) s2)
+  | tLambda s0 s1 s2 =>
+      congr_tLambda (eq_refl s0) (extRen_term xi_term zeta_term Eq_term s1)
+        (extRen_term (upRen_term_term xi_term) (upRen_term_term zeta_term)
+           (upExtRen_term_term _ _ Eq_term) s2)
+  | tApp s0 s1 =>
+      congr_tApp (extRen_term xi_term zeta_term Eq_term s0)
+        (extRen_term xi_term zeta_term Eq_term s1)
+  end.
+
+Lemma upExt_term_term (sigma : nat -> term) (tau : nat -> term)
+  (Eq : forall x, sigma x = tau x) :
+  forall x, up_term_term sigma x = up_term_term tau x.
+Proof.
+exact (fun n =>
+       match n with
+       | S n' => ap (ren_term shift) (Eq n')
+       | O => eq_refl
+       end).
+Qed.
+
+Fixpoint ext_term (sigma_term : nat -> term) (tau_term : nat -> term)
+(Eq_term : forall x, sigma_term x = tau_term x) (s : term) {struct s} :
+subst_term sigma_term s = subst_term tau_term s :=
+  match s with
+  | tRel s0 => Eq_term s0
+  | tSort s0 => congr_tSort (eq_refl s0)
+  | tProd s0 s1 s2 =>
+      congr_tProd (eq_refl s0) (ext_term sigma_term tau_term Eq_term s1)
+        (ext_term (up_term_term sigma_term) (up_term_term tau_term)
+           (upExt_term_term _ _ Eq_term) s2)
+  | tLambda s0 s1 s2 =>
+      congr_tLambda (eq_refl s0) (ext_term sigma_term tau_term Eq_term s1)
+        (ext_term (up_term_term sigma_term) (up_term_term tau_term)
+           (upExt_term_term _ _ Eq_term) s2)
+  | tApp s0 s1 =>
+      congr_tApp (ext_term sigma_term tau_term Eq_term s0)
+        (ext_term sigma_term tau_term Eq_term s1)
+  end.
+
+Lemma up_ren_ren_term_term (xi : nat -> nat) (zeta : nat -> nat)
+  (rho : nat -> nat) (Eq : forall x, funcomp zeta xi x = rho x) :
+  forall x,
+  funcomp (upRen_term_term zeta) (upRen_term_term xi) x =
+  upRen_term_term rho x.
+Proof.
+exact (up_ren_ren xi zeta rho Eq).
+Qed.
+
+Fixpoint compRenRen_term (xi_term : nat -> nat) (zeta_term : nat -> nat)
+(rho_term : nat -> nat)
+(Eq_term : forall x, funcomp zeta_term xi_term x = rho_term x) (s : term)
+{struct s} : ren_term zeta_term (ren_term xi_term s) = ren_term rho_term s :=
+  match s with
+  | tRel s0 => ap (tRel) (Eq_term s0)
+  | tSort s0 => congr_tSort (eq_refl s0)
+  | tProd s0 s1 s2 =>
+      congr_tProd (eq_refl s0)
+        (compRenRen_term xi_term zeta_term rho_term Eq_term s1)
+        (compRenRen_term (upRen_term_term xi_term)
+           (upRen_term_term zeta_term) (upRen_term_term rho_term)
+           (up_ren_ren _ _ _ Eq_term) s2)
+  | tLambda s0 s1 s2 =>
+      congr_tLambda (eq_refl s0)
+        (compRenRen_term xi_term zeta_term rho_term Eq_term s1)
+        (compRenRen_term (upRen_term_term xi_term)
+           (upRen_term_term zeta_term) (upRen_term_term rho_term)
+           (up_ren_ren _ _ _ Eq_term) s2)
+  | tApp s0 s1 =>
+      congr_tApp (compRenRen_term xi_term zeta_term rho_term Eq_term s0)
+        (compRenRen_term xi_term zeta_term rho_term Eq_term s1)
+  end.
+
+Lemma up_ren_subst_term_term (xi : nat -> nat) (tau : nat -> term)
+  (theta : nat -> term) (Eq : forall x, funcomp tau xi x = theta x) :
+  forall x,
+  funcomp (up_term_term tau) (upRen_term_term xi) x = up_term_term theta x.
+Proof.
+exact (fun n =>
+       match n with
+       | S n' => ap (ren_term shift) (Eq n')
+       | O => eq_refl
+       end).
+Qed.
+
+Fixpoint compRenSubst_term (xi_term : nat -> nat) (tau_term : nat -> term)
+(theta_term : nat -> term)
+(Eq_term : forall x, funcomp tau_term xi_term x = theta_term x) (s : term)
+{struct s} :
+subst_term tau_term (ren_term xi_term s) = subst_term theta_term s :=
+  match s with
+  | tRel s0 => Eq_term s0
+  | tSort s0 => congr_tSort (eq_refl s0)
+  | tProd s0 s1 s2 =>
+      congr_tProd (eq_refl s0)
+        (compRenSubst_term xi_term tau_term theta_term Eq_term s1)
+        (compRenSubst_term (upRen_term_term xi_term) (up_term_term tau_term)
+           (up_term_term theta_term) (up_ren_subst_term_term _ _ _ Eq_term)
+           s2)
+  | tLambda s0 s1 s2 =>
+      congr_tLambda (eq_refl s0)
+        (compRenSubst_term xi_term tau_term theta_term Eq_term s1)
+        (compRenSubst_term (upRen_term_term xi_term) (up_term_term tau_term)
+           (up_term_term theta_term) (up_ren_subst_term_term _ _ _ Eq_term)
+           s2)
+  | tApp s0 s1 =>
+      congr_tApp (compRenSubst_term xi_term tau_term theta_term Eq_term s0)
+        (compRenSubst_term xi_term tau_term theta_term Eq_term s1)
+  end.
+
+Lemma up_subst_ren_term_term (sigma : nat -> term) (zeta_term : nat -> nat)
+  (theta : nat -> term)
+  (Eq : forall x, funcomp (ren_term zeta_term) sigma x = theta x) :
+  forall x,
+  funcomp (ren_term (upRen_term_term zeta_term)) (up_term_term sigma) x =
+  up_term_term theta x.
+Proof.
+exact (fun n =>
+       match n with
+       | S n' =>
+           eq_trans
+             (compRenRen_term shift (upRen_term_term zeta_term)
+                (funcomp shift zeta_term) (fun x => eq_refl) (sigma n'))
+             (eq_trans
+                (eq_sym
+                   (compRenRen_term zeta_term shift (funcomp shift zeta_term)
+                      (fun x => eq_refl) (sigma n')))
+                (ap (ren_term shift) (Eq n')))
+       | O => eq_refl
+       end).
+Qed.
+
+Fixpoint compSubstRen_term (sigma_term : nat -> term)
+(zeta_term : nat -> nat) (theta_term : nat -> term)
+(Eq_term : forall x, funcomp (ren_term zeta_term) sigma_term x = theta_term x)
+(s : term) {struct s} :
+ren_term zeta_term (subst_term sigma_term s) = subst_term theta_term s :=
+  match s with
+  | tRel s0 => Eq_term s0
+  | tSort s0 => congr_tSort (eq_refl s0)
+  | tProd s0 s1 s2 =>
+      congr_tProd (eq_refl s0)
+        (compSubstRen_term sigma_term zeta_term theta_term Eq_term s1)
+        (compSubstRen_term (up_term_term sigma_term)
+           (upRen_term_term zeta_term) (up_term_term theta_term)
+           (up_subst_ren_term_term _ _ _ Eq_term) s2)
+  | tLambda s0 s1 s2 =>
+      congr_tLambda (eq_refl s0)
+        (compSubstRen_term sigma_term zeta_term theta_term Eq_term s1)
+        (compSubstRen_term (up_term_term sigma_term)
+           (upRen_term_term zeta_term) (up_term_term theta_term)
+           (up_subst_ren_term_term _ _ _ Eq_term) s2)
+  | tApp s0 s1 =>
+      congr_tApp
+        (compSubstRen_term sigma_term zeta_term theta_term Eq_term s0)
+        (compSubstRen_term sigma_term zeta_term theta_term Eq_term s1)
+  end.
+
+Lemma up_subst_subst_term_term (sigma : nat -> term) (tau_term : nat -> term)
+  (theta : nat -> term)
+  (Eq : forall x, funcomp (subst_term tau_term) sigma x = theta x) :
+  forall x,
+  funcomp (subst_term (up_term_term tau_term)) (up_term_term sigma) x =
+  up_term_term theta x.
+Proof.
+exact (fun n =>
+       match n with
+       | S n' =>
+           eq_trans
+             (compRenSubst_term shift (up_term_term tau_term)
+                (funcomp (up_term_term tau_term) shift) (fun x => eq_refl)
+                (sigma n'))
+             (eq_trans
+                (eq_sym
+                   (compSubstRen_term tau_term shift
+                      (funcomp (ren_term shift) tau_term) (fun x => eq_refl)
+                      (sigma n'))) (ap (ren_term shift) (Eq n')))
+       | O => eq_refl
+       end).
+Qed.
+
+Fixpoint compSubstSubst_term (sigma_term : nat -> term)
+(tau_term : nat -> term) (theta_term : nat -> term)
+(Eq_term : forall x,
+           funcomp (subst_term tau_term) sigma_term x = theta_term x)
+(s : term) {struct s} :
+subst_term tau_term (subst_term sigma_term s) = subst_term theta_term s :=
+  match s with
+  | tRel s0 => Eq_term s0
+  | tSort s0 => congr_tSort (eq_refl s0)
+  | tProd s0 s1 s2 =>
+      congr_tProd (eq_refl s0)
+        (compSubstSubst_term sigma_term tau_term theta_term Eq_term s1)
+        (compSubstSubst_term (up_term_term sigma_term)
+           (up_term_term tau_term) (up_term_term theta_term)
+           (up_subst_subst_term_term _ _ _ Eq_term) s2)
+  | tLambda s0 s1 s2 =>
+      congr_tLambda (eq_refl s0)
+        (compSubstSubst_term sigma_term tau_term theta_term Eq_term s1)
+        (compSubstSubst_term (up_term_term sigma_term)
+           (up_term_term tau_term) (up_term_term theta_term)
+           (up_subst_subst_term_term _ _ _ Eq_term) s2)
+  | tApp s0 s1 =>
+      congr_tApp
+        (compSubstSubst_term sigma_term tau_term theta_term Eq_term s0)
+        (compSubstSubst_term sigma_term tau_term theta_term Eq_term s1)
+  end.
+
+Lemma renRen_term (xi_term : nat -> nat) (zeta_term : nat -> nat) (s : term)
+  :
+  ren_term zeta_term (ren_term xi_term s) =
+  ren_term (funcomp zeta_term xi_term) s.
+Proof.
+exact (compRenRen_term xi_term zeta_term _ (fun n => eq_refl) s).
+Qed.
+
+Lemma renRen'_term_pointwise (xi_term : nat -> nat) (zeta_term : nat -> nat)
+  :
+  pointwise_relation _ eq (funcomp (ren_term zeta_term) (ren_term xi_term))
+    (ren_term (funcomp zeta_term xi_term)).
+Proof.
+exact (fun s => compRenRen_term xi_term zeta_term _ (fun n => eq_refl) s).
+Qed.
+
+Lemma renSubst_term (xi_term : nat -> nat) (tau_term : nat -> term)
+  (s : term) :
+  subst_term tau_term (ren_term xi_term s) =
+  subst_term (funcomp tau_term xi_term) s.
+Proof.
+exact (compRenSubst_term xi_term tau_term _ (fun n => eq_refl) s).
+Qed.
+
+Lemma renSubst_term_pointwise (xi_term : nat -> nat) (tau_term : nat -> term)
+  :
+  pointwise_relation _ eq (funcomp (subst_term tau_term) (ren_term xi_term))
+    (subst_term (funcomp tau_term xi_term)).
+Proof.
+exact (fun s => compRenSubst_term xi_term tau_term _ (fun n => eq_refl) s).
+Qed.
+
+Lemma substRen_term (sigma_term : nat -> term) (zeta_term : nat -> nat)
+  (s : term) :
+  ren_term zeta_term (subst_term sigma_term s) =
+  subst_term (funcomp (ren_term zeta_term) sigma_term) s.
+Proof.
+exact (compSubstRen_term sigma_term zeta_term _ (fun n => eq_refl) s).
+Qed.
+
+Lemma substRen_term_pointwise (sigma_term : nat -> term)
+  (zeta_term : nat -> nat) :
+  pointwise_relation _ eq
+    (funcomp (ren_term zeta_term) (subst_term sigma_term))
+    (subst_term (funcomp (ren_term zeta_term) sigma_term)).
+Proof.
+exact (fun s => compSubstRen_term sigma_term zeta_term _ (fun n => eq_refl) s).
+Qed.
+
+Lemma substSubst_term (sigma_term : nat -> term) (tau_term : nat -> term)
+  (s : term) :
+  subst_term tau_term (subst_term sigma_term s) =
+  subst_term (funcomp (subst_term tau_term) sigma_term) s.
+Proof.
+exact (compSubstSubst_term sigma_term tau_term _ (fun n => eq_refl) s).
+Qed.
+
+Lemma substSubst_term_pointwise (sigma_term : nat -> term)
+  (tau_term : nat -> term) :
+  pointwise_relation _ eq
+    (funcomp (subst_term tau_term) (subst_term sigma_term))
+    (subst_term (funcomp (subst_term tau_term) sigma_term)).
+Proof.
+exact (fun s =>
+       compSubstSubst_term sigma_term tau_term _ (fun n => eq_refl) s).
+Qed.
+
+Lemma rinstInst_up_term_term (xi : nat -> nat) (sigma : nat -> term)
+  (Eq : forall x, funcomp (tRel) xi x = sigma x) :
+  forall x, funcomp (tRel) (upRen_term_term xi) x = up_term_term sigma x.
+Proof.
+exact (fun n =>
+       match n with
+       | S n' => ap (ren_term shift) (Eq n')
+       | O => eq_refl
+       end).
+Qed.
+
+Fixpoint rinst_inst_term (xi_term : nat -> nat) (sigma_term : nat -> term)
+(Eq_term : forall x, funcomp (tRel) xi_term x = sigma_term x) (s : term)
+{struct s} : ren_term xi_term s = subst_term sigma_term s :=
+  match s with
+  | tRel s0 => Eq_term s0
+  | tSort s0 => congr_tSort (eq_refl s0)
+  | tProd s0 s1 s2 =>
+      congr_tProd (eq_refl s0)
+        (rinst_inst_term xi_term sigma_term Eq_term s1)
+        (rinst_inst_term (upRen_term_term xi_term) (up_term_term sigma_term)
+           (rinstInst_up_term_term _ _ Eq_term) s2)
+  | tLambda s0 s1 s2 =>
+      congr_tLambda (eq_refl s0)
+        (rinst_inst_term xi_term sigma_term Eq_term s1)
+        (rinst_inst_term (upRen_term_term xi_term) (up_term_term sigma_term)
+           (rinstInst_up_term_term _ _ Eq_term) s2)
+  | tApp s0 s1 =>
+      congr_tApp (rinst_inst_term xi_term sigma_term Eq_term s0)
+        (rinst_inst_term xi_term sigma_term Eq_term s1)
+  end.
+
+Lemma rinstInst'_term (xi_term : nat -> nat) (s : term) :
+  ren_term xi_term s = subst_term (funcomp (tRel) xi_term) s.
+Proof.
+exact (rinst_inst_term xi_term _ (fun n => eq_refl) s).
+Qed.
+
+Lemma rinstInst'_term_pointwise (xi_term : nat -> nat) :
+  pointwise_relation _ eq (ren_term xi_term)
+    (subst_term (funcomp (tRel) xi_term)).
+Proof.
+exact (fun s => rinst_inst_term xi_term _ (fun n => eq_refl) s).
+Qed.
+
+Lemma instId'_term (s : term) : subst_term (tRel) s = s.
+Proof.
+exact (idSubst_term (tRel) (fun n => eq_refl) s).
+Qed.
+
+Lemma instId'_term_pointwise :
+  pointwise_relation _ eq (subst_term (tRel)) id.
+Proof.
+exact (fun s => idSubst_term (tRel) (fun n => eq_refl) s).
+Qed.
+
+Lemma rinstId'_term (s : term) : ren_term id s = s.
+Proof.
+exact (eq_ind_r (fun t => t = s) (instId'_term s) (rinstInst'_term id s)).
+Qed.
+
+Lemma rinstId'_term_pointwise : pointwise_relation _ eq (@ren_term id) id.
+Proof.
+exact (fun s =>
+       eq_ind_r (fun t => t = s) (instId'_term s) (rinstInst'_term id s)).
+Qed.
+
+Lemma varL'_term (sigma_term : nat -> term) (x : nat) :
+  subst_term sigma_term (tRel x) = sigma_term x.
+Proof.
+exact (eq_refl).
+Qed.
+
+Lemma varL'_term_pointwise (sigma_term : nat -> term) :
+  pointwise_relation _ eq (funcomp (subst_term sigma_term) (tRel))
+    sigma_term.
+Proof.
+exact (fun x => eq_refl).
+Qed.
+
+Lemma varLRen'_term (xi_term : nat -> nat) (x : nat) :
+  ren_term xi_term (tRel x) = tRel (xi_term x).
+Proof.
+exact (eq_refl).
+Qed.
+
+Lemma varLRen'_term_pointwise (xi_term : nat -> nat) :
+  pointwise_relation _ eq (funcomp (ren_term xi_term) (tRel))
+    (funcomp (tRel) xi_term).
+Proof.
+exact (fun x => eq_refl).
+Qed.
+
+Class Up_term X Y :=
+    up_term : X -> Y.
+
+#[global] Instance Subst_term : (Subst1 _ _ _) := @subst_term.
+
+#[global] Instance Up_term_term : (Up_term _ _) := @up_term_term.
+
+#[global] Instance Ren_term : (Ren1 _ _ _) := @ren_term.
+
+#[global] Instance VarInstance_term : (Var _ _) := @tRel.
+
+Notation "[ sigma_term ]" := (subst_term sigma_term)
+  ( at level 1, left associativity, only printing) : fscope.
+
+Notation "s [ sigma_term ]" := (subst_term sigma_term s)
+  ( at level 7, left associativity, only printing) : subst_scope.
+
+Notation "↑__term" := up_term (only printing) : subst_scope.
+
+Notation "↑__term" := up_term_term (only printing) : subst_scope.
+
+Notation "⟨ xi_term ⟩" := (ren_term xi_term)
+  ( at level 1, left associativity, only printing) : fscope.
+
+Notation "s ⟨ xi_term ⟩" := (ren_term xi_term s)
+  ( at level 7, left associativity, only printing) : subst_scope.
+
+Notation "'var'" := tRel ( at level 1, only printing) : subst_scope.
+
+Notation "x '__term'" := (@ids _ _ VarInstance_term x)
+  ( at level 5, format "x __term", only printing) : subst_scope.
+
+Notation "x '__term'" := (tRel x) ( at level 5, format "x __term") :
+  subst_scope.
+
+#[global] Instance subst_term_morphism :
+ (Proper (respectful (pointwise_relation _ eq) (respectful eq eq))
+    (@subst_term)).
+Proof.
+exact (fun f_term g_term Eq_term s t Eq_st =>
+       eq_ind s (fun t' => subst_term f_term s = subst_term g_term t')
+         (ext_term f_term g_term Eq_term s) t Eq_st).
+Qed.
+
+#[global] Instance subst_term_morphism2 :
+ (Proper (respectful (pointwise_relation _ eq) (pointwise_relation _ eq))
+    (@subst_term)).
+Proof.
+exact (fun f_term g_term Eq_term s => ext_term f_term g_term Eq_term s).
+Qed.
+
+#[global] Instance ren_term_morphism :
+ (Proper (respectful (pointwise_relation _ eq) (respectful eq eq))
+    (@ren_term)).
+Proof.
+exact (fun f_term g_term Eq_term s t Eq_st =>
+       eq_ind s (fun t' => ren_term f_term s = ren_term g_term t')
+         (extRen_term f_term g_term Eq_term s) t Eq_st).
+Qed.
+
+#[global] Instance ren_term_morphism2 :
+ (Proper (respectful (pointwise_relation _ eq) (pointwise_relation _ eq))
+    (@ren_term)).
+Proof.
+exact (fun f_term g_term Eq_term s => extRen_term f_term g_term Eq_term s).
+Qed.
+
+Ltac auto_unfold := repeat
+                     unfold VarInstance_term, Var, ids, Ren_term, Ren1, ren1,
+                      Up_term_term, Up_term, up_term, Subst_term, Subst1,
+                      subst1.
+
+Tactic Notation "auto_unfold" "in" "*" := repeat
+                                           unfold VarInstance_term, Var, ids,
+                                            Ren_term, Ren1, ren1,
+                                            Up_term_term, Up_term, up_term,
+                                            Subst_term, Subst1, subst1 
+                                            in *.
+
+Ltac asimpl' := repeat (first
+                 [ progress setoid_rewrite substSubst_term_pointwise
+                 | progress setoid_rewrite substSubst_term
+                 | progress setoid_rewrite substRen_term_pointwise
+                 | progress setoid_rewrite substRen_term
+                 | progress setoid_rewrite renSubst_term_pointwise
+                 | progress setoid_rewrite renSubst_term
+                 | progress setoid_rewrite renRen'_term_pointwise
+                 | progress setoid_rewrite renRen_term
+                 | progress setoid_rewrite varLRen'_term_pointwise
+                 | progress setoid_rewrite varLRen'_term
+                 | progress setoid_rewrite varL'_term_pointwise
+                 | progress setoid_rewrite varL'_term
+                 | progress setoid_rewrite rinstId'_term_pointwise
+                 | progress setoid_rewrite rinstId'_term
+                 | progress setoid_rewrite instId'_term_pointwise
+                 | progress setoid_rewrite instId'_term
+                 | progress unfold up_term_term, upRen_term_term, up_ren
+                 | progress cbn[subst_term ren_term]
+                 | progress fsimpl ]).
+
+Ltac asimpl := check_no_evars;
+                repeat
+                 unfold VarInstance_term, Var, ids, Ren_term, Ren1, ren1,
+                  Up_term_term, Up_term, up_term, Subst_term, Subst1, subst1
+                  in *; asimpl'; minimize.
+
+Tactic Notation "asimpl" "in" hyp(J) := revert J; asimpl; intros J.
+
+Tactic Notation "auto_case" := auto_case ltac:(asimpl; cbn; eauto).
+
+Ltac substify := auto_unfold; try setoid_rewrite rinstInst'_term_pointwise;
+                  try setoid_rewrite rinstInst'_term.
+
+Ltac renamify := auto_unfold;
+                  try setoid_rewrite_left rinstInst'_term_pointwise;
+                  try setoid_rewrite_left rinstInst'_term.
+
+End Core.
+
+Module Allfv.
+
+Import
+Core.
+
+Lemma upAllfv_term_term (p : nat -> Prop) : nat -> Prop.
+Proof.
+exact (up_allfv p).
+Defined.
+
+Fixpoint allfv_term (p_term : nat -> Prop) (s : term) {struct s} : Prop :=
+  match s with
+  | tRel s0 => p_term s0
+  | tSort s0 => and True True
+  | tProd s0 s1 s2 =>
+      and True
+        (and (allfv_term p_term s1)
+           (and (allfv_term (upAllfv_term_term p_term) s2) True))
+  | tLambda s0 s1 s2 =>
+      and True
+        (and (allfv_term p_term s1)
+           (and (allfv_term (upAllfv_term_term p_term) s2) True))
+  | tApp s0 s1 =>
+      and (allfv_term p_term s0) (and (allfv_term p_term s1) True)
+  end.
+
+Lemma upAllfvTriv_term_term {p : nat -> Prop} (H : forall x, p x) :
+  forall x, upAllfv_term_term p x.
+Proof.
+exact (fun x => match x with
+                | S n' => H n'
+                | O => I
+                end).
+Qed.
+
+Fixpoint allfvTriv_term (p_term : nat -> Prop) (H_term : forall x, p_term x)
+(s : term) {struct s} : allfv_term p_term s :=
+  match s with
+  | tRel s0 => H_term s0
+  | tSort s0 => conj I I
+  | tProd s0 s1 s2 =>
+      conj I
+        (conj (allfvTriv_term p_term H_term s1)
+           (conj
+              (allfvTriv_term (upAllfv_term_term p_term)
+                 (upAllfvTriv_term_term H_term) s2) I))
+  | tLambda s0 s1 s2 =>
+      conj I
+        (conj (allfvTriv_term p_term H_term s1)
+           (conj
+              (allfvTriv_term (upAllfv_term_term p_term)
+                 (upAllfvTriv_term_term H_term) s2) I))
+  | tApp s0 s1 =>
+      conj (allfvTriv_term p_term H_term s0)
+        (conj (allfvTriv_term p_term H_term s1) I)
+  end.
+
+Lemma upAllfvImpl_term_term {p : nat -> Prop} {q : nat -> Prop}
+  (H : forall x, p x -> q x) :
+  forall x, upAllfv_term_term p x -> upAllfv_term_term q x.
+Proof.
+exact (fun x => match x with
+                | S n' => H n'
+                | O => fun Hp => Hp
+                end).
+Qed.
+
+Fixpoint allfvImpl_term (p_term : nat -> Prop) (q_term : nat -> Prop)
+(H_term : forall x, p_term x -> q_term x) (s : term) {struct s} :
+allfv_term p_term s -> allfv_term q_term s :=
+  match s with
+  | tRel s0 => fun HP => H_term s0 HP
+  | tSort s0 => fun HP => conj I I
+  | tProd s0 s1 s2 =>
+      fun HP =>
+      conj I
+        (conj
+           (allfvImpl_term p_term q_term H_term s1
+              match HP with
+              | conj _ HP => match HP with
+                             | conj HP _ => HP
+                             end
+              end)
+           (conj
+              (allfvImpl_term (upAllfv_term_term p_term)
+                 (upAllfv_term_term q_term) (upAllfvImpl_term_term H_term) s2
+                 match HP with
+                 | conj _ HP =>
+                     match HP with
+                     | conj _ HP => match HP with
+                                    | conj HP _ => HP
+                                    end
+                     end
+                 end) I))
+  | tLambda s0 s1 s2 =>
+      fun HP =>
+      conj I
+        (conj
+           (allfvImpl_term p_term q_term H_term s1
+              match HP with
+              | conj _ HP => match HP with
+                             | conj HP _ => HP
+                             end
+              end)
+           (conj
+              (allfvImpl_term (upAllfv_term_term p_term)
+                 (upAllfv_term_term q_term) (upAllfvImpl_term_term H_term) s2
+                 match HP with
+                 | conj _ HP =>
+                     match HP with
+                     | conj _ HP => match HP with
+                                    | conj HP _ => HP
+                                    end
+                     end
+                 end) I))
+  | tApp s0 s1 =>
+      fun HP =>
+      conj
+        (allfvImpl_term p_term q_term H_term s0
+           match HP with
+           | conj HP _ => HP
+           end)
+        (conj
+           (allfvImpl_term p_term q_term H_term s1
+              match HP with
+              | conj _ HP => match HP with
+                             | conj HP _ => HP
+                             end
+              end) I)
+  end.
+
+Lemma upAllfvRenL_term_term (p : nat -> Prop) (xi : nat -> nat) :
+  forall x,
+  upAllfv_term_term p (upRen_term_term xi x) ->
+  upAllfv_term_term (funcomp p xi) x.
+Proof.
+exact (fun x => match x with
+                | S n' => fun i => i
+                | O => fun H => H
+                end).
+Qed.
+
+Fixpoint allfvRenL_term (p_term : nat -> Prop) (xi_term : nat -> nat)
+(s : term) {struct s} :
+allfv_term p_term (ren_term xi_term s) ->
+allfv_term (funcomp p_term xi_term) s :=
+  match s with
+  | tRel s0 => fun H => H
+  | tSort s0 => fun H => conj I I
+  | tProd s0 s1 s2 =>
+      fun H =>
+      conj I
+        (conj
+           (allfvRenL_term p_term xi_term s1
+              match H with
+              | conj _ H => match H with
+                            | conj H _ => H
+                            end
+              end)
+           (conj
+              (allfvImpl_term _ _ (upAllfvRenL_term_term p_term xi_term) s2
+                 (allfvRenL_term (upAllfv_term_term p_term)
+                    (upRen_term_term xi_term) s2
+                    match H with
+                    | conj _ H =>
+                        match H with
+                        | conj _ H => match H with
+                                      | conj H _ => H
+                                      end
+                        end
+                    end)) I))
+  | tLambda s0 s1 s2 =>
+      fun H =>
+      conj I
+        (conj
+           (allfvRenL_term p_term xi_term s1
+              match H with
+              | conj _ H => match H with
+                            | conj H _ => H
+                            end
+              end)
+           (conj
+              (allfvImpl_term _ _ (upAllfvRenL_term_term p_term xi_term) s2
+                 (allfvRenL_term (upAllfv_term_term p_term)
+                    (upRen_term_term xi_term) s2
+                    match H with
+                    | conj _ H =>
+                        match H with
+                        | conj _ H => match H with
+                                      | conj H _ => H
+                                      end
+                        end
+                    end)) I))
+  | tApp s0 s1 =>
+      fun H =>
+      conj
+        (allfvRenL_term p_term xi_term s0 match H with
+                                          | conj H _ => H
+                                          end)
+        (conj
+           (allfvRenL_term p_term xi_term s1
+              match H with
+              | conj _ H => match H with
+                            | conj H _ => H
+                            end
+              end) I)
+  end.
+
+Lemma upAllfvRenR_term_term (p : nat -> Prop) (xi : nat -> nat) :
+  forall x,
+  upAllfv_term_term (funcomp p xi) x ->
+  upAllfv_term_term p (upRen_term_term xi x).
+Proof.
+exact (fun x => match x with
+                | S n' => fun i => i
+                | O => fun H => H
+                end).
+Qed.
+
+Fixpoint allfvRenR_term (p_term : nat -> Prop) (xi_term : nat -> nat)
+(s : term) {struct s} :
+allfv_term (funcomp p_term xi_term) s ->
+allfv_term p_term (ren_term xi_term s) :=
+  match s with
+  | tRel s0 => fun H => H
+  | tSort s0 => fun H => conj I I
+  | tProd s0 s1 s2 =>
+      fun H =>
+      conj I
+        (conj
+           (allfvRenR_term p_term xi_term s1
+              match H with
+              | conj _ H => match H with
+                            | conj H _ => H
+                            end
+              end)
+           (conj
+              (allfvRenR_term (upAllfv_term_term p_term)
+                 (upRen_term_term xi_term) s2
+                 (allfvImpl_term _ _ (upAllfvRenR_term_term p_term xi_term)
+                    s2
+                    match H with
+                    | conj _ H =>
+                        match H with
+                        | conj _ H => match H with
+                                      | conj H _ => H
+                                      end
+                        end
+                    end)) I))
+  | tLambda s0 s1 s2 =>
+      fun H =>
+      conj I
+        (conj
+           (allfvRenR_term p_term xi_term s1
+              match H with
+              | conj _ H => match H with
+                            | conj H _ => H
+                            end
+              end)
+           (conj
+              (allfvRenR_term (upAllfv_term_term p_term)
+                 (upRen_term_term xi_term) s2
+                 (allfvImpl_term _ _ (upAllfvRenR_term_term p_term xi_term)
+                    s2
+                    match H with
+                    | conj _ H =>
+                        match H with
+                        | conj _ H => match H with
+                                      | conj H _ => H
+                                      end
+                        end
+                    end)) I))
+  | tApp s0 s1 =>
+      fun H =>
+      conj
+        (allfvRenR_term p_term xi_term s0 match H with
+                                          | conj H _ => H
+                                          end)
+        (conj
+           (allfvRenR_term p_term xi_term s1
+              match H with
+              | conj _ H => match H with
+                            | conj H _ => H
+                            end
+              end) I)
+  end.
+
+End Allfv.
+
+Module Extra.
+
+Import Core.
+
+#[export]Hint Opaque subst_term: rewrite.
+
+#[export]Hint Opaque ren_term: rewrite.
+
+End Extra.
+
+Module interface.
+
+Export Core.
+
+Export Allfv.
+
+Export Extra.
+
+End interface.
+
+Export interface.
+
