theories/BasicAst.v
@@ -1,0 +1,17 @@
+From Coq Require Import String Bool.
+From LogRel.AutoSubst Require Import core unscoped.
+
+Record aname := { nNamed : string }.
+
+Definition eq_binder_annot (a a' : aname) :=
+  String.eqb a.(nNamed) a'.(nNamed).
+
+Lemma eq_binder_annot_eq a a' : reflect (a = a') (eq_binder_annot a a').
+Proof.
+  destruct a as [a], a' as [a'] ; cbn.
+  destruct (String.eqb_spec a a').
+  all: constructor ; congruence.
+Qed.
+
+Inductive sort :=
+  | set : sort.
