theories/Context.v
@@ -1,0 +1,63 @@
+From Coq Require Import ssreflect Morphisms Setoid.
+From LogRel.AutoSubst Require Import core unscoped Ast.
+From LogRel Require Import Utils BasicAst.
+
+Import UnscopedNotations.
+#[local] Open Scope subst_scope.
+
+(** *** The context of De Bruijn indices *)
+
+Record context_decl := mkdecl {
+  decl_name : aname ;
+  decl_type : term
+}.
+
+Definition map_decl (f : term -> term) : context_decl -> context_decl :=
+  fun d => {| decl_name := d.(decl_name) ; decl_type := f d.(decl_type) |}.
+
+Lemma map_decl_id (f : term -> term) : f =1 id -> map_decl f =1 id.
+Proof.
+  intros Hf [a t].
+  cbv.
+  f_equal.
+  now apply Hf.
+Qed.
+
+Lemma compose_map_decl f g x :
+  map_decl f (map_decl g x) = map_decl (g >> f) x.
+Proof.
+  destruct x; reflexivity.
+Qed.
+
+Lemma map_decl_ext f g x : (forall x, f x = g x) -> map_decl f x = map_decl g x.
+Proof.
+  intros H; destruct x; rewrite /map_decl /=; f_equal; auto.
+Qed.
+
+#[global] Instance map_decl_proper : Proper (`=1` ==> Logic.eq ==> Logic.eq) map_decl.
+Proof.
+  intros f g Hfg x y ->. now apply map_decl_ext.
+Qed.
+
+#[global] Instance map_decl_pointwise : Proper (`=1` ==> `=1`) map_decl.
+Proof. intros f g Hfg x. rewrite /map_decl.
+  destruct x => /=. f_equal.
+  now rewrite Hfg.
+Qed.
+
+Arguments map_decl _%fscope.
+
+#[global] Instance Ren_decl : (Ren1 (nat -> nat) context_decl context_decl) :=
+  fun ρ t => map_decl (ren_term ρ) t.
+
+Definition vass a A := {| decl_name := a ; decl_type := A |}.
+
+Definition context := list context_decl.
+
+Notation "'ε'" := (@nil context_decl).
+Notation " Γ ,, d " := (@cons context_decl d Γ) (at level 20, d at next level).
+Notation " Γ ,,, Δ " := (@app context_decl Δ Γ) (at level 25, Δ at next level, left associativity).
+
+Inductive in_ctx : context -> nat -> context_decl -> Type :=
+  | in_here Γ d : in_ctx (Γ,,d) 0 (d⟨↑⟩)
+  | in_there Γ d d' n : in_ctx Γ n d -> in_ctx (Γ,,d') (S n) (map_decl (ren_term shift) d).
