theories/Utils.v
@@ -1,0 +1,16 @@
+From Coq Require Import Morphisms List.
+From MetaCoq Require Export MCPrelude MCProd.
+From LogRel.AutoSubst Require Import core.
+
+Notation "#| l |" := (List.length l) (at level 0, l at level 99, format "#| l |").
+Notation "`=1`" := (pointwise_relation _ Logic.eq) (at level 80).
+Infix "=1" := (pointwise_relation _ Logic.eq) (at level 70).
+Notation "`=2`" := (pointwise_relation _ (pointwise_relation _ Logic.eq)) (at level 80).
+Infix "=2" := (pointwise_relation _ (pointwise_relation _ Logic.eq)) (at level 70).
+
+(* The database used for generic typing *)
+Create HintDb gen_typing.
+#[global] Hint Constants Opaque : gen_typing.
+#[global] Hint Variables Transparent : gen_typing.
+
+Ltac gen_typing := typeclasses eauto 6 with gen_typing typeclass_instances.
